Fix decidability of Ollvm_ast.value

src/coq/DecidableEquality.v
@@ -8,7 +8,8 @@ Require Import compcert.lib.Integers.
 Require Import Vellvm.Ollvm_ast Vellvm.CFG Vellvm.StepSemantics Vellvm.Memory.
 Require Import Vellvm.Classes.
 Require Import Vellvm.AstLib.
-
+Require Import Vellvm.Util.
+Require Import List.
 (** ** Decidable Equality *) 
 
 Instance eq_dec_int : eq_dec (BinNums.Z) := Z.eq_dec.
@@ -24,7 +25,7 @@ Ltac lift_decide_eq :=
     try lift_decide_eq
   | |- { ?C ?x = ?C ?y} + { ~(?C ?x = ?C ?y) } =>
     destruct (decide (x = y));
-    [subst; auto | right; discriminate_goal]
+      [subst; auto | right; discriminate_goal]
   | |- { ?C ?x1 ?x2 = ?C ?y1 ?y2} + { ~(?C ?x1 ?x2 = ?C ?y1 ?y2) } =>
     try (destruct (decide (x1 = y1));
          [subst; auto | right; discriminate_goal]);
@@ -73,7 +74,7 @@ Ltac lift_decide_eq_from_inside_dv :=
          [subst; auto | right; discriminate_goal]);
     try (destruct (decide (x2 = y2));
          [subst; auto | right; discriminate_goal])
-  | |- { DV (?C ?x1 ?x2 ?x3) = DV (?C ?y1 ?y2 ?y3)} +
+  | |- { DV (?C ?x1 ?x2 ?x3) = DV (?Cd ?y1 ?y2 ?y3)} +
       { ~(DV (?C ?x1 ?x2 ?x3) = DV (?C ?y1 ?y2 ?y3)) } =>
     try (destruct (decide (x1 = y1));
          [subst; auto | right; discriminate_goal]);
@@ -309,15 +310,512 @@ Proof.
   lift_decide_eq; left; auto.
 Defined.
 
-(*
-Instance decide_expr {A : Set} `{decide_value : eq_dec A} : eq_dec (Expr A).
+Definition value_ind': forall (P : Ollvm_ast.value  -> Set),
+    (forall id : ident, P (VALUE_Ident id)) ->
+    (forall x : int, P (VALUE_Integer x)) ->
+    (forall f : float, P (VALUE_Float f)) ->
+    (forall h : String.string, P (VALUE_Hex h)) ->    
+    (forall b : bool, P (VALUE_Bool b)) ->
+    (P VALUE_Null) ->
+    (P VALUE_Zero_initializer) ->
+    (forall s : String.string, P (VALUE_Cstring s)) ->
+    (P VALUE_Undef) ->
+    (P (VALUE_Struct [])) ->
+    (forall t v fields,
+        P v ->
+        P (VALUE_Struct fields) ->
+        P (VALUE_Struct ((t, v) :: fields))) ->
+    (P (VALUE_Packed_struct [])) ->
+    (forall t v fields,
+        P v ->
+        P (VALUE_Packed_struct fields) ->
+        P (VALUE_Packed_struct ((t, v) :: fields))) ->
+    (P (VALUE_Array [])) ->
+    (forall t v arr,
+        P v ->
+        P (VALUE_Array arr) ->
+        P (VALUE_Array ((t, v) :: arr))) ->
+    (P (VALUE_Vector [])) ->
+    (forall t v vec,
+        P v ->
+        P (VALUE_Vector vec) ->
+        P (VALUE_Vector ((t, v) :: vec))) ->
+    (forall iop t v1 v2,
+        P v1 -> P v2 ->
+        P (OP_IBinop iop t v1 v2)) ->
+    (forall cmp t v1 v2,
+        P v1 -> P v2 ->
+        P (OP_ICmp cmp t v1 v2)) ->
+    (forall fop fm t v1 v2,
+        P v1 -> P v2 ->
+        P (OP_FBinop fop fm t v1 v2)) ->
+    (forall cmp t v1 v2,
+        P v1 -> P v2 ->
+        P (OP_FCmp cmp t v1 v2)) ->
+    (forall conv t_from v t_to,
+        P v -> P (OP_Conversion conv t_from v t_to)) ->
+    (forall t ptr_t ptr_v,
+        P ptr_v ->
+        P (OP_GetElementPtr t (ptr_t, ptr_v) [])) ->
+    (forall t ptr_t ptr_v idx_t idx_v indices,
+        P ptr_v ->
+        P idx_v ->
+        P (OP_GetElementPtr t (ptr_t, ptr_v) indices) ->
+        P (OP_GetElementPtr t (ptr_t, ptr_v) ((idx_t, idx_v) :: indices))) ->
+    (forall vec_t vec_v idx_t idx_v,
+        P vec_v -> P idx_v -> P (OP_ExtractElement (vec_t, vec_v) (idx_t, idx_v))) ->
+    (forall vec_t vec_v elt_t elt_v idx_t idx_v,
+        P vec_v -> P elt_v -> P idx_v ->
+        P (OP_InsertElement (vec_t, vec_v) (elt_t, elt_v) (idx_t, idx_v))) ->
+    (forall vec1_t vec1_v vec2_t vec2_v idxmask_t idxmask_v,
+        P vec1_v -> P vec2_v -> P (idxmask_v) ->
+        P (OP_ShuffleVector (vec1_t, vec1_v) (vec2_t, vec2_v) (idxmask_t, idxmask_v))) ->
+    (forall vec_t vec_v idxs,
+        P vec_v -> P (OP_ExtractValue (vec_t, vec_v) idxs)) ->
+    (forall vec_t vec_v elt_t elt_v idxs,
+        P vec_v -> P elt_v ->
+        P (OP_InsertValue (vec_t, vec_v) (elt_t, elt_v) idxs)) ->
+    (forall cnd_t cnd_v v1_t v1_v v2_t v2_v,
+        P cnd_v -> P v1_v -> P v2_v ->
+        P (OP_Select (cnd_t, cnd_v) (v1_t, v1_v) (v2_t, v2_v))) ->
+    (forall v : Ollvm_ast.value , P v).
 Proof.
-  destruct x; destruct y; unfold Decidable;
+  intros P H_Ident H_Integer H_Float H_Hex H_Bool H_Null
+         H_Zero_initializer H_Cstring H_Undef.
+  intros IH_Struct_Base IH_Struct_Ind
+         IH_Packed_struct_Base IH_Packed_struct_Ind
+         IH_Array_Base IH_Array_Ind
+         IH_Vector_Base IH_Vector_Ind
+         IH_IBinop IH_ICmp IH_FBinop IH_FCmp
+         IH_Conversion
+         IH_GetElementPtr_Base IH_GetElementPtr_Ind
+         IH_ExtractElement IH_InsertElement
+         IH_ShuffleVector IH_ExtractValue IH_InsertValue
+         IH_Select.
+
+  refine
+    (fix prove_dv (v : Ollvm_ast.value ) :=
+       match v with
+         | VALUE_Ident id => _
+         | VALUE_Integer n => _
+         | VALUE_Float f => _
+         | VALUE_Hex h => _                             
+         | VALUE_Bool b => _
+         | VALUE_Null => _
+         | VALUE_Zero_initializer => _
+         | VALUE_Cstring s => _
+         | VALUE_Undef => _
+         | VALUE_Struct l =>
+           let
+             fix prove_l (l : list (Ollvm_ast.typ * Ollvm_ast.value)) :=
+             match l with
+             | [] => IH_Struct_Base
+             | (t, v) :: rest =>
+               IH_Struct_Ind t v rest (prove_dv v) (prove_l rest)
+             end
+           in prove_l l 
+         | VALUE_Packed_struct l =>
+           let
+             fix prove_l (l : list (Ollvm_ast.typ * Ollvm_ast.value)) :=
+             match l with
+             | [] => IH_Packed_struct_Base
+             | (t, v) :: rest =>
+               IH_Packed_struct_Ind t v rest (prove_dv v) (prove_l rest)
+             end
+           in prove_l l 
+         | VALUE_Array l =>
+           let
+             fix prove_l (l : list (Ollvm_ast.typ * Ollvm_ast.value)) :=
+             match l with
+             | [] => IH_Array_Base
+             | (t, v) :: rest =>
+               IH_Array_Ind t v rest (prove_dv v) (prove_l rest)
+             end
+           in prove_l l 
+
+         | VALUE_Vector l =>
+           let
+             fix prove_l (l : list (Ollvm_ast.typ * Ollvm_ast.value)) :=
+             match l with
+             | [] => IH_Vector_Base
+             | (t, v) :: rest =>
+               IH_Vector_Ind t v rest (prove_dv v) (prove_l rest)
+             end
+           in prove_l l            
+
+         | OP_IBinop op t v1 v2 =>
+           IH_IBinop op t v1 v2 (prove_dv v1) (prove_dv v2) 
+         | OP_ICmp op t v1 v2 => 
+           IH_ICmp op t v1 v2 (prove_dv v1) (prove_dv v2) 
+         | OP_FBinop op fm t v1 v2 =>
+           IH_FBinop op fm t v1 v2 (prove_dv v1) (prove_dv v2) 
+         | OP_FCmp op t v1 v2 =>
+           IH_FCmp op t v1 v2 (prove_dv v1) (prove_dv v2) 
+         | OP_Conversion conv t_from v t_to =>
+           IH_Conversion conv t_from v t_to (prove_dv v)
+           
+         | OP_GetElementPtr t (ptr_t, ptr_v) l =>
+           let fix prove_l (l : list (Ollvm_ast.typ * Ollvm_ast.value)) :=
+               match l with
+               | [] =>
+                 IH_GetElementPtr_Base t ptr_t ptr_v (prove_dv ptr_v)
+               | (idx_t, idx_v) :: rest =>
+                 IH_GetElementPtr_Ind t ptr_t ptr_v idx_t idx_v rest
+                                      (prove_dv ptr_v) (prove_dv idx_v)
+                                      (prove_l rest)
+               end
+           in prove_l l
+           
+         | OP_ExtractElement (vec_t, vec_v) (idx_t, idx_v) =>
+           IH_ExtractElement vec_t vec_v idx_t idx_v
+                             (prove_dv vec_v) (prove_dv idx_v)
+         | OP_InsertElement (vec_t, vec_v) (elt_t, elt_v) (idx_t, idx_v) =>
+           IH_InsertElement vec_t vec_v elt_t elt_v idx_t idx_v
+                            (prove_dv vec_v) (prove_dv elt_v) (prove_dv idx_v)
+         | OP_ShuffleVector (vec1_t, vec1_v) (vec2_t, vec2_v) (idxmask_t, idxmask_v) => 
+           IH_ShuffleVector vec1_t vec1_v vec2_t vec2_v idxmask_t idxmask_v
+                            (prove_dv vec1_v) (prove_dv vec2_v) (prove_dv idxmask_v)
+         | OP_ExtractValue (vec_t, vec_v) idxs =>
+           IH_ExtractValue vec_t vec_v idxs (prove_dv vec_v) 
+         | OP_InsertValue (vec_t, vec_v) (elt_t, elt_v) idxs =>
+           IH_InsertValue vec_t vec_v elt_t elt_v idxs
+                          (prove_dv vec_v) (prove_dv elt_v)
+         | OP_Select (cnd_t, cnd_v) (v1_t, v1_v) (v2_t, v2_v) =>
+           IH_Select cnd_t cnd_v v1_t v1_v v2_t v2_v
+                     (prove_dv cnd_v) (prove_dv v1_v) (prove_dv v2_v)
+         end
+    ); auto.
+Defined.
+
+Instance decide_value : eq_dec (Ollvm_ast.value).
+Proof.
+  induction x using value_ind'; destruct y; unfold Decidable;
     try (right; intro H; inversion H; tauto);
     try (left; reflexivity);
     try (lift_decide_eq).
+   
+  (* Case Value_Struct *)
+  - destruct fields; auto.
+  - refine
+      (match fields0 with
+       | [] => right _
+       | (t', v') :: fields' =>
+         match (decide (t = t')) with
+         | left t_eq =>
+           match decide (x = v') with
+           | left value_eq =>
+             match decide ((VALUE_Struct fields) =
+                           (VALUE_Struct fields')) with
+             | left fields_eq => left _
+             | right fields_neq => right _
+             end
+           | right value_neq => right _
+           end
+         | right t_neq => right _
+         end
+       end).
+
+    { intros H; inversion H. }
+    { inversion fields_eq. subst. reflexivity. }
+    { intros H; inversion H; apply fields_neq; subst; auto. }
+    { intros H; inversion H; apply value_neq; subst; auto. }
+    { intros H; inversion H; apply t_neq; subst; auto. }
+
+    (* (VALUE_Packed_struct ...) *)
+  - destruct fields; auto.
+  - refine
+      (match fields0 with
+       | [] => right _
+       | (t', v') :: fields' =>
+         match (decide (t = t')) with
+         | left t_eq =>
+           match decide (x = v') with
+           | left value_eq =>
+             match decide ((VALUE_Packed_struct fields) =
+                           (VALUE_Packed_struct fields')) with
+             | left fields_eq => left _
+             | right fields_neq => right _
+             end
+           | right value_neq => right _
+           end
+         | right t_neq => right _
+         end
+       end).
+    { intros H; inversion H. }
+    { inversion fields_eq. subst. reflexivity. }
+    { intros H; inversion H; apply fields_neq; subst; auto. }
+    { intros H; inversion H; apply value_neq; subst; auto. }
+    { intros H; inversion H; apply t_neq; subst; auto. }
+
+    (* (VALUE_Array ...) *)
+  - destruct elts; auto.
+  - destruct elts as [| (t', x') arr']; auto.
+    refine
+      (match (decide (t = t')) with
+       | left t_eq =>
+         match (decide (x = x')) with
+         | left value_eq =>
+           match decide ((VALUE_Array arr) = (VALUE_Array arr')) with
+           | left rest_eq => left _
+           | right rest_neq => right _
+           end
+         | right value_neq => right _
+         end
+       | right t_neq => right _
+       end).
+    { inversion rest_eq; subst; auto. }
+    { intros H; inversion H; apply rest_neq; subst; auto. }
+    { intros H; inversion H; apply value_neq; subst; auto. }
+    { intros H; inversion H; apply t_neq; subst; auto. }
+
+    (* DV (VALUE_Vector *)
+  - destruct elts; auto.
+  - destruct elts as [| (t', x') vec']; auto.
+    refine
+      (match (decide (t = t')) with
+       | left t_eq =>
+         match (decide (x = x')) with
+         | left value_eq =>
+           match decide ((VALUE_Vector vec) = (VALUE_Vector vec')) with
+           | left rest_eq => left _
+           | right rest_neq => right _
+           end
+         | right value_neq => right _
+         end
+       | right t_neq => right _
+       end).
+    { inversion rest_eq; subst; auto. }
+    { intros H; inversion H; apply rest_neq; subst; auto. }
+    { intros H; inversion H; apply value_neq; subst; auto. }
+    { intros H; inversion H; apply t_neq; subst; auto. }
+
+
+    (* OP_GetElementPtr ... *)
+  - destruct ptrval as (ptr_t', ptr_v');
+      destruct idxs; try (right; intros H; inversion H; tauto).
+    refine
+      (match decide (ptr_t = ptr_t') with
+       | left t_eq =>
+         match decide (x = ptr_v') with
+         | left ptr_value_eq => left _
+         | right ptr_value_neq => right _
+         end
+       | right t_neq => right _
+       end).
+    { subst; reflexivity. } 
+    { intros H; inversion H; apply ptr_value_neq; subst; auto. }
+    { intros H; inversion H; apply t_neq; subst; auto. }
+  - destruct ptrval as (ptr_t', ptr_v');
+      destruct idxs as [| (idx_t', idx_v')];
+      try (right; intros H; inversion H; tauto).
+    refine
+      (match decide (ptr_t = ptr_t') with
+       | left ptr_t_eq =>
+         match decide (x1 = ptr_v') with
+         | left ptr_value_eq =>
+           match decide (idx_t = idx_t') with
+           | left idx_t_eq =>
+             match decide (x2 = idx_v') with
+             | left idx_value_eq => _
+             | right idx_value_neq => right _
+             end
+           | right idx_t_neq => right _
+           end
+         | right ptr_value_neq => right _
+         end
+       | right t_neq => right _
+       end).
+    { subst.
+      refine
+        (match decide ((OP_GetElementPtr t0 (ptr_t', ptr_v') indices) =
+                       (OP_GetElementPtr t0 (ptr_t', ptr_v') idxs)) with
+         | left rest_eq => left _
+         | right rest_neq => right _
+         end).
+      { inversion rest_eq; subst; auto. }
+      { intros H; inversion H; apply rest_neq; subst; auto. }
+    }
+    { intros H; inversion H; apply idx_value_neq; subst; auto. }
+    { intros H; inversion H; apply idx_t_neq; subst; auto. }
+    { intros H; inversion H; apply ptr_value_neq; subst; auto. }
+    { intros H; inversion H; apply t_neq; subst; auto. }
+
+    (* (OP_ExtractElement ...), arity 2 *)
+  - destruct vec as (vec_t', vec_v');
+      destruct idx as (idx_t', idx_v');
+      try (right; intros H; inversion H; tauto).
+    refine (match decide (vec_t = vec_t') with
+            | left vec_t_eq =>
+              match decide (x1 = vec_v') with
+              | left vec_v_eq =>
+                match decide (idx_t = idx_t') with
+                | left idx_t_eq =>
+                  match decide (x2 = idx_v') with
+                  | left idx_v_eq => left _
+                  | right idx_v_neq => right _
+                  end
+                | right idx_t_neq => right _
+                end
+              | right vec_v_neq => right _
+              end
+            | right vec_t_neq => right _
+            end); subst; auto.
+    { intros H; inversion H; apply idx_v_neq; subst; auto. }
+    { intros H; inversion H; apply idx_t_neq; subst; auto. }
+    { intros H; inversion H; apply vec_v_neq; subst; auto. }
+    { intros H; inversion H; apply vec_t_neq; subst; auto. }
+
+
+    (* DV (OP_InsertElement ...), arity 3 *)
+  - destruct vec as (vec_t', vec_v');
+      destruct elt as (elt_t', elt_v');      
+      destruct idx as (idx_t', idx_v');
+      try (right; intros H; inversion H; tauto).
+    refine (match decide (vec_t = vec_t') with
+            | left vec_t_eq =>
+              match decide (x1 = vec_v') with
+              | left vec_v_eq =>
+                match decide (elt_t = elt_t') with
+                | left elt_t_eq =>
+                  match decide (x2 = elt_v') with
+                  | left elt_v_eq => 
+                    match decide (idx_t = idx_t') with
+                    | left idx_t_eq =>
+                      match decide (x3 = idx_v') with
+                      | left idx_v_eq => left _
+                      | right idx_v_neq => right _
+                      end
+                    | right idx_t_neq => right _
+                    end
+                  | right elt_v_neq => right _
+                  end
+                | right elt_t_neq => right _
+                end                  
+              | right vec_v_neq => right _
+              end
+            | right vec_t_neq => right _
+            end); subst; auto.
+    { intros H; inversion H; apply idx_v_neq; subst; auto. }
+    { intros H; inversion H; apply idx_t_neq; subst; auto. }
+    { intros H; inversion H; apply elt_v_neq; subst; auto. }
+    { intros H; inversion H; apply elt_t_neq; subst; auto. }
+    { intros H; inversion H; apply vec_v_neq; subst; auto. }
+    { intros H; inversion H; apply vec_t_neq; subst; auto. }
+
+    (* (OP_ShuffleVector ...) ; Same as (OP_InsertElement ...), with arity 3 *)
+  - destruct vec1 as (vec1_t', vec1_v');
+      destruct vec2 as (vec2_t', vec2_v');      
+      destruct idxmask as (idxmask_t', idxmask_v');
+      try (right; intros H; inversion H; tauto).
+    refine (match decide (vec1_t = vec1_t') with
+            | left vec1_t_eq =>
+              match decide (x1 = vec1_v') with
+              | left vec1_v_eq =>
+                match decide (vec2_t = vec2_t') with
+                | left vec2_t_eq =>
+                  match decide (x2 = vec2_v') with
+                  | left vec2_v_eq => 
+                    match decide (idxmask_t = idxmask_t') with
+                    | left idxmask_t_eq =>
+                      match decide (x3 = idxmask_v') with
+                      | left idxmask_v_eq => left _
+                      | right idxmask_v_neq => right _
+                      end
+                    | right idxmask_t_neq => right _
+                    end
+                  | right vec2_v_neq => right _
+                  end
+                | right vec2_t_neq => right _
+                end                  
+              | right vec1_v_neq => right _
+              end
+            | right vec1_t_neq => right _
+            end); subst; auto.
+    { intros H; inversion H; apply idxmask_v_neq; subst; auto. }
+    { intros H; inversion H; apply idxmask_t_neq; subst; auto. }
+    { intros H; inversion H; apply vec2_v_neq; subst; auto. }
+    { intros H; inversion H; apply vec2_t_neq; subst; auto. }
+    { intros H; inversion H; apply vec1_v_neq; subst; auto. }
+    { intros H; inversion H; apply vec1_t_neq; subst; auto. }
+
+    (* OP_ExtractValue ... ; Same as OP_ *)
+  - destruct vec as (vec_t', vec_v');
+      try (right; intros H; inversion H; tauto).
+    refine
+      (match decide (vec_t = vec_t') with
+       | left t_eq =>
+         match decide (x = vec_v') with
+         | left v_eq => left _
+         | right v_neq => right _
+         end
+       | right t_neq => right _
+       end); subst; auto.
+    { intros H; inversion H; apply v_neq; subst; auto. }
+    { intros H; inversion H; apply t_neq; subst; auto. }
+
+    (* OP_InsertValue ... *)
+  - destruct vec as (vec_t', vec_v');
+      destruct elt as (elt_t', elt_v');
+      try (right; intros H; inversion H; tauto).
+    refine (match decide (vec_t = vec_t') with
+            | left vec_t_eq =>
+              match decide (x1 = vec_v') with
+              | left vec_v_eq =>
+                match decide (elt_t = elt_t') with
+                | left elt_t_eq =>
+                  match decide (x2 = elt_v') with
+                  | left elt_v_eq => left _
+                  | right elt_v_neq => right _
+                  end
+                | right elt_t_neq => right _
+                end
+              | right vec_v_neq => right _
+              end
+            | right vec_t_neq => right _
+            end); subst; auto.
+    { intros H; inversion H; apply elt_v_neq; subst; auto. }
+    { intros H; inversion H; apply elt_t_neq; subst; auto. }
+    { intros H; inversion H; apply vec_v_neq; subst; auto. }
+    { intros H; inversion H; apply vec_t_neq; subst; auto. }
+
+    (* OP_Select ... *)
+  - destruct cnd as (cnd_t', cnd_v');
+      destruct v1 as (v1_t', v1_v');
+      destruct v2 as (v2_t', v2_v');
+      try (right; intros H; inversion H; tauto).
+    refine (match decide (cnd_t = cnd_t') with
+            | left cnd_t_eq =>
+              match decide (x1 = cnd_v') with
+              | left cnd_v_eq =>
+                match decide (v1_t = v1_t') with
+                | left v1_t_eq =>
+                  match decide (x2 = v1_v') with
+                  | left v1_v_eq => 
+                    match decide (v2_t = v2_t') with
+                    | left v2_t_eq =>
+                      match decide (x3 = v2_v') with
+                      | left v2_v_eq => left _
+                      | right v2_v_neq => right _
+                      end
+                    | right v2_t_neq => right _
+                    end
+                  | right v1_v_neq => right _
+                  end
+                | right v1_t_neq => right _
+                end                  
+              | right cnd_v_neq => right _
+              end
+            | right cnd_t_neq => right _
+            end); subst; auto.
+    { intros H; inversion H; apply v2_v_neq; subst; auto. }
+    { intros H; inversion H; apply v2_t_neq; subst; auto. }
+    { intros H; inversion H; apply v1_v_neq; subst; auto. }
+    { intros H; inversion H; apply v1_t_neq; subst; auto. }
+    { intros H; inversion H; apply cnd_v_neq; subst; auto. }
+    { intros H; inversion H; apply cnd_t_neq; subst; auto. }
 Defined.
 
+(*
 Definition expr_dvalue_ind: forall (P : dvalue -> Set),
     (forall id : ident, P (DV (VALUE_Ident id))) ->
     (forall x : int, P (DV (VALUE_Integer x))) ->
@@ -514,16 +1012,17 @@ Proof.
        end
     ); auto.
 Defined.  
-*)
-(*
+
+Instance eq_dec_lldouble : eq_dec ll_double := Floats.Float.eq_dec.
+Instance eq_dec_llfloat : eq_dec ll_float := Floats.Float32.eq_dec.
+
 Instance eq_dvalue : eq_dec dvalue.
 Proof.
-  induction x using expr_dvalue_ind; destruct y; 
+  induction x; destruct y; 
     try (right; intro H; inversion H; tauto);
     try (lift_decide_eq);
     try destruct e; unfold Decidable;
       try (right; intro H; inversion H; tauto);
-      try (lift_decide_eq_from_inside_dv);
       try solve [left; auto];
       try solve [lift_decide_eq].
 
@@ -620,229 +1119,6 @@ Proof.
     { intros H; inversion H; apply rest_neq; subst; auto. }
     { intros H; inversion H; apply value_neq; subst; auto. }
     { intros H; inversion H; apply t_neq; subst; auto. }
-
-    (* DV (OP_GetElementPtr ...) *)
-  - destruct ptrval as (ptr_t', ptr_v');
-      destruct idxs; try (right; intros H; inversion H; tauto).
-    refine
-      (match decide (ptr_t = ptr_t') with
-       | left t_eq =>
-         match decide (x = ptr_v') with
-         | left ptr_value_eq => left _
-         | right ptr_value_neq => right _
-         end
-       | right t_neq => right _
-       end).
-    { subst; reflexivity. } 
-    { intros H; inversion H; apply ptr_value_neq; subst; auto. }
-    { intros H; inversion H; apply t_neq; subst; auto. }
-  - destruct ptrval as (ptr_t', ptr_v');
-      destruct idxs as [| (idx_t', idx_v')];
-      try (right; intros H; inversion H; tauto).
-    refine
-      (match decide (ptr_t = ptr_t') with
-       | left ptr_t_eq =>
-         match decide (x1 = ptr_v') with
-         | left ptr_value_eq =>
-           match decide (idx_t = idx_t') with
-           | left idx_t_eq =>
-             match decide (x2 = idx_v') with
-             | left idx_value_eq => _
-             | right idx_value_neq => right _
-             end
-           | right idx_t_neq => right _
-           end
-         | right ptr_value_neq => right _
-         end
-       | right t_neq => right _
-       end).
-    { subst.
-      refine
-        (match decide (DV (OP_GetElementPtr t0 (ptr_t', ptr_v') indices) =
-                       DV (OP_GetElementPtr t0 (ptr_t', ptr_v') idxs)) with
-         | left rest_eq => left _
-         | right rest_neq => right _
-         end).
-      { inversion rest_eq; subst; auto. }
-      { intros H; inversion H; apply rest_neq; subst; auto. }
-    }
-    { intros H; inversion H; apply idx_value_neq; subst; auto. }
-    { intros H; inversion H; apply idx_t_neq; subst; auto. }
-    { intros H; inversion H; apply ptr_value_neq; subst; auto. }
-    { intros H; inversion H; apply t_neq; subst; auto. }
-
-    (* DV (OP_ExtractElement ...), arity 2 *)
-  - destruct vec as (vec_t', vec_v');
-      destruct idx as (idx_t', idx_v');
-      try (right; intros H; inversion H; tauto).
-    refine (match decide (vec_t = vec_t') with
-            | left vec_t_eq =>
-              match decide (x1 = vec_v') with
-              | left vec_v_eq =>
-                match decide (idx_t = idx_t') with
-                | left idx_t_eq =>
-                  match decide (x2 = idx_v') with
-                  | left idx_v_eq => left _
-                  | right idx_v_neq => right _
-                  end
-                | right idx_t_neq => right _
-                end
-              | right vec_v_neq => right _
-              end
-            | right vec_t_neq => right _
-            end); subst; auto.
-    { intros H; inversion H; apply idx_v_neq; subst; auto. }
-    { intros H; inversion H; apply idx_t_neq; subst; auto. }
-    { intros H; inversion H; apply vec_v_neq; subst; auto. }
-    { intros H; inversion H; apply vec_t_neq; subst; auto. }
-
-    (* DV (OP_InsertElement ...), arity 3 *)
-  - destruct vec as (vec_t', vec_v');
-      destruct elt as (elt_t', elt_v');      
-      destruct idx as (idx_t', idx_v');
-      try (right; intros H; inversion H; tauto).
-    refine (match decide (vec_t = vec_t') with
-            | left vec_t_eq =>
-              match decide (x1 = vec_v') with
-              | left vec_v_eq =>
-                match decide (elt_t = elt_t') with
-                | left elt_t_eq =>
-                  match decide (x2 = elt_v') with
-                  | left elt_v_eq => 
-                    match decide (idx_t = idx_t') with
-                    | left idx_t_eq =>
-                      match decide (x3 = idx_v') with
-                      | left idx_v_eq => left _
-                      | right idx_v_neq => right _
-                      end
-                    | right idx_t_neq => right _
-                    end
-                  | right elt_v_neq => right _
-                  end
-                | right elt_t_neq => right _
-                end                  
-              | right vec_v_neq => right _
-              end
-            | right vec_t_neq => right _
-            end); subst; auto.
-    { intros H; inversion H; apply idx_v_neq; subst; auto. }
-    { intros H; inversion H; apply idx_t_neq; subst; auto. }
-    { intros H; inversion H; apply elt_v_neq; subst; auto. }
-    { intros H; inversion H; apply elt_t_neq; subst; auto. }    
-    { intros H; inversion H; apply vec_v_neq; subst; auto. }
-    { intros H; inversion H; apply vec_t_neq; subst; auto. }
-
-    (* DV (OP_ShuffleVector ...) ; Same as DV (OP_InsertElement ...), with arity 3 *)
-  - destruct vec1 as (vec1_t', vec1_v');
-      destruct vec2 as (vec2_t', vec2_v');      
-      destruct idxmask as (idxmask_t', idxmask_v');
-      try (right; intros H; inversion H; tauto).
-    refine (match decide (vec1_t = vec1_t') with
-            | left vec1_t_eq =>
-              match decide (x1 = vec1_v') with
-              | left vec1_v_eq =>
-                match decide (vec2_t = vec2_t') with
-                | left vec2_t_eq =>
-                  match decide (x2 = vec2_v') with
-                  | left vec2_v_eq => 
-                    match decide (idxmask_t = idxmask_t') with
-                    | left idxmask_t_eq =>
-                      match decide (x3 = idxmask_v') with
-                      | left idxmask_v_eq => left _
-                      | right idxmask_v_neq => right _
-                      end
-                    | right idxmask_t_neq => right _
-                    end
-                  | right vec2_v_neq => right _
-                  end
-                | right vec2_t_neq => right _
-                end                  
-              | right vec1_v_neq => right _
-              end
-            | right vec1_t_neq => right _
-            end); subst; auto.
-    { intros H; inversion H; apply idxmask_v_neq; subst; auto. }
-    { intros H; inversion H; apply idxmask_t_neq; subst; auto. }
-    { intros H; inversion H; apply vec2_v_neq; subst; auto. }
-    { intros H; inversion H; apply vec2_t_neq; subst; auto. }    
-    { intros H; inversion H; apply vec1_v_neq; subst; auto. }
-    { intros H; inversion H; apply vec1_t_neq; subst; auto. }
-
-    (* DV (OP_ExtractValue ...) ; Same as DV (OP_ *)
-  - destruct vec as (vec_t', vec_v');
-      try (right; intros H; inversion H; tauto).
-    refine
-      (match decide (vec_t = vec_t') with
-       | left t_eq =>
-         match decide (x = vec_v') with
-         | left v_eq => left _
-         | right v_neq => right _
-         end
-       | right t_neq => right _
-       end); subst; auto.
-    { intros H; inversion H; apply v_neq; subst; auto. }
-    { intros H; inversion H; apply t_neq; subst; auto. }
-
-    (* DV (OP_InsertValue ...) *)
-  - destruct vec as (vec_t', vec_v');
-      destruct elt as (elt_t', elt_v');
-      try (right; intros H; inversion H; tauto).
-    refine (match decide (vec_t = vec_t') with
-            | left vec_t_eq =>
-              match decide (x1 = vec_v') with
-              | left vec_v_eq =>
-                match decide (elt_t = elt_t') with
-                | left elt_t_eq =>
-                  match decide (x2 = elt_v') with
-                  | left elt_v_eq => left _
-                  | right elt_v_neq => right _
-                  end
-                | right elt_t_neq => right _
-                end
-              | right vec_v_neq => right _
-              end
-            | right vec_t_neq => right _
-            end); subst; auto.
-    { intros H; inversion H; apply elt_v_neq; subst; auto. }
-    { intros H; inversion H; apply elt_t_neq; subst; auto. }
-    { intros H; inversion H; apply vec_v_neq; subst; auto. }
-    { intros H; inversion H; apply vec_t_neq; subst; auto. }
-
-    (* DV (OP_Select ...) *)
-  - destruct cnd as (cnd_t', cnd_v');
-      destruct v1 as (v1_t', v1_v');
-      destruct v2 as (v2_t', v2_v');
-      try (right; intros H; inversion H; tauto).
-    refine (match decide (cnd_t = cnd_t') with
-            | left cnd_t_eq =>
-              match decide (x1 = cnd_v') with
-              | left cnd_v_eq =>
-                match decide (v1_t = v1_t') with
-                | left v1_t_eq =>
-                  match decide (x2 = v1_v') with
-                  | left v1_v_eq => 
-                    match decide (v2_t = v2_t') with
-                    | left v2_t_eq =>
-                      match decide (x3 = v2_v') with
-                      | left v2_v_eq => left _
-                      | right v2_v_neq => right _
-                      end
-                    | right v2_t_neq => right _
-                    end
-                  | right v1_v_neq => right _
-                  end
-                | right v1_t_neq => right _
-                end                  
-              | right cnd_v_neq => right _
-              end
-            | right cnd_t_neq => right _
-            end); subst; auto.
-    { intros H; inversion H; apply v2_v_neq; subst; auto. }
-    { intros H; inversion H; apply v2_t_neq; subst; auto. }
-    { intros H; inversion H; apply v1_v_neq; subst; auto. }
-    { intros H; inversion H; apply v1_t_neq; subst; auto. }    
-    { intros H; inversion H; apply cnd_v_neq; subst; auto. }
-    { intros H; inversion H; apply cnd_t_neq; subst; auto. }
 Defined.
 *)
 
